src/tls/StatefulLHAE.fst
@@ -18,6 +18,9 @@ open Range
 open LHAEPlain
 open AEAD_GCM
 open StatefulPlain
+open MonotoneSeq
+open FStar.Monotonic.RRef
+module HH = HyperHeap
 
 type id = AEAD_GCM.gid //TODO: TEMPORARY, until we add back LHAE 
 
@@ -32,9 +35,6 @@ type dplain (i:id) (ad:adata i) (c:cipher i) =
 type entry (i:id) = (* records that c is an encryption of p with ad *)
   | Entry: c:cipher i -> ad:adata i -> p:dplain i ad c -> entry i
 
-let is_seqn (n:nat) = repr_bytes n <= 8
-let seqn_t = n:nat { repr_bytes n <= 8 } (* NB: REMOVING THIS LINE TRIGGERS A FATAL ERROR WHEN CHECKING writer_seqn; NS: Stale?*)
-
 (* typing the log that specifies StatefulLHAE *)
 type st_log_t (r:rid) (i:id) = rref r (s:seq (entry i))
 
@@ -48,7 +48,7 @@ type state (i:gid) (rw:rw) =
     -> peer_region:rid{peer_region <> root 
                         /\ HyperHeap.disjoint region peer_region}
     -> log:  st_log_t (if rw=Reader then peer_region else region) i (* shared ghost spec *)
-    -> seqn: rref region seqn_t                                       (* concrete, local sequence number *)
+    -> seqn: rref region seqn                                       (* concrete, local sequence number *)
     -> key:  AEAD_GCM.state i rw{extends key.region region /\ extends key.peer_region peer_region} (* gcm in a distinct sub-region *)
     -> state i rw
 
@@ -66,7 +66,7 @@ let log_region    = fun (#i:id) (#rw:rw) (s:state i rw) -> if rw=Reader then pee
 abstract val log: #i:id -> #rw:rw -> s:state i rw -> Tot (st_log_t (log_region s) i)
 let log #i #rw s = s.log
 
-abstract val seqn: #i:id -> #rw:rw -> s:state i rw -> Tot (rref (region s) seqn_t)
+abstract val seqn: #i:id -> #rw:rw -> s:state i rw -> Tot (rref (region s) seqn)
 let seqn #i #rw s = s.seqn
 
 abstract type matching (#i:gid) (r:reader i) (w:writer i) =
